actually fixed question 5

Assignment1/Ex5.dfy
@@ -5,52 +5,39 @@
 //				   September 2019						   //
 /////////////////////////////////////////////////////////////
 
-// Ex5.dfy 6 marks. 
-// An array is even-odd sorted if the array consists of 
+// Ex5.dfy 6 marks.
+// An array is even-odd sorted if the array consists of
 // even-sorted and odd-sorted sub-arrays.
-// An even-sorted sub-array is an array in which 
+// An even-sorted sub-array is an array in which
 // all the values at even indexes are sorted. Analogously
-// for an odd-sorted sub-array. 
+// for an odd-sorted sub-array.
 
 // An example is:
 // [2,1,4,2,6,3]
-// In this array, the even-sorted sub-array is [2,4,6], 
-// the odd-sorted sub-array is [1,2,3] 
+// In this array, the even-sorted sub-array is [2,4,6],
+// the odd-sorted sub-array is [1,2,3]
 // The arrays [1,2], [2,1] and [] are even-odd sorted.
 // The array [1,2,3,1] is not even-odd sorted.
-// Write a Dafny predicate called EOSorted that, given an array, 
+// Write a Dafny predicate called EOSorted that, given an array,
 // is true if the array is even-odd sorted, and
-// false otherwise. Test the predicate behaves correctly 
+// false otherwise. Test the predicate behaves correctly
 // by writing a method Test that calls the predicate
 // for all the testcases mentioned above.
 
-method EOSorted(a: array<int>) returns(IsEoSorted:bool)
+predicate EOSorted(a: array<int>)
 requires a !=  null
-ensures a.Length >= 0 && a.Length <= 2 ==> true
-// if all even + odd pairs are sorted return true post conidtion 
-ensures if forall i,j :: 0 <= i <= j < a.Length - 2 && j == i+2 && (a[i] < a[j]) then true else false;
+reads a
+// if all even + odd pairs are sorted return true post conidtion
+ensures forall i,j :: 0 <= i <= j < a.Length - 2 && j == i+2 && (a[i] < a[j]) 
+==> true ==> exists i,j :: 0 <= i <= j < a.Length - 2 && j == i+2 && (a[i] > a[j]) ==> false;
 // doesn't modify array post condition
-ensures forall i :: 0 <= i < a.Length ==> a[i] == old(a[i]) 
 {
-    IsEoSorted := true;
-    if(a.Length > 2){
-        var i := 0;
-        while i < a.Length - 2
-        invariant 0 <= i <= a.Length - 2
-        {
-            if(a[i] > a[i+2]){
-                IsEoSorted := false;
-                return;
-            }
-            i := i + 1;
-        }
-    }else{
-        IsEoSorted := true;
-    } 
-    //assert forall i,j :: 0 <= i <= j < a.Length - 2 && j == i+2 && (a[i] < a[j]) ==> (IsEoSorted == true);
+    forall i,j :: 0 <= i <= j < a.Length - 2 && j == i+2 ==> a[i] < a[j] 
+    ==> !exists i,j :: 0 <= i <= j < a.Length - 2 && j == i+2 && (a[i] > a[j])
+    
 }
 
-method Main()
+method Test()
 {
     var testArray1: array<int> := new int[6];
     testArray1[0], testArray1[1], testArray1[2],testArray1[3],testArray1[4], testArray1[5] := 2, 1, 4, 2, 6, 3;
@@ -66,20 +53,20 @@ method Main()
     var testArray5: array<int> := new int[4];
     testArray5[0], testArray5[1], testArray5[2],testArray5[3] := 1, 2, 3, 1;
 
-    var test1 := EOSorted(testArray1);
-    //assert test1 == true;
+    assert EOSorted(testArray1);
+    //assert test1 == false;
 
-    var test2 := EOSorted(testArray2);
+    assert EOSorted(testArray2);
     //assert test2 == true;
 
-    var test3 := EOSorted(testArray3);
+    assert EOSorted(testArray3);
     //assert test3 == true;
 
-    var test4 := EOSorted(testArray4);
+    assert EOSorted(testArray4);
     //assert test4 == true;
 
-    var test5 := EOSorted(testArray5);
+    assert EOSorted(testArray5);
     //assert test5 == false;
 
-    print test1, "--", test2, "--", test3, "--",test4, "--",test5, "--\n";
+    //print test1, "--", test2, "--", test3, "--",test4, "--",test5, "--\n";
 }
